Implement stop requests (#1)

Runtime/Network/Execution/Basic.lean
@@ -5,24 +5,28 @@ structure Reactor {net : Network} (cls : Class net) where
   interface : (kind : Reactor.InterfaceKind) → kind.interfaceType (cls.interface kind)
   timer : cls.timers → Timer
 
-namespace Network
+namespace Network.Executable
 
-def Executable.LawfulQueue (queue : Array (Event net)) (time : Time) := 
+def LawfulQueue (queue : Array (Event net)) (time : Time) := 
   ∀ {event}, (queue[0]? = some event) → event.time ≥ time
 
-theorem Executable.LawfulQueue.merge :
+theorem LawfulQueue.merge :
   (LawfulQueue queue₁ time) → (LawfulQueue queue₂ time) → (LawfulQueue (queue₁.merge queue₂) time) :=
   sorry
 
-structure Executable (net : Network) where
+inductive State
+  | executing
+  | stopRequested
+  | shuttingDown 
+  deriving DecidableEq
+
+structure _root_.Network.Executable (net : Network) where
   tag : Tag := ⟨0, 0⟩
   physicalOffset : Duration
   queue : Array (Event net)
   reactors : (id : ReactorId net) → Reactor id.class
-  isShuttingDown : Bool := false
-  lawfulQueue : Executable.LawfulQueue queue tag.time
-
-namespace Executable
+  state : State := .executing
+  lawfulQueue : LawfulQueue queue tag.time
 
 def isStartingUp (exec : Executable net) : Bool := 
   exec.tag = ⟨0, 0⟩
@@ -36,6 +40,4 @@ def interface (exec : Executable net) (id : ReactorId net) :=
 def timer (exec : Executable net) (id : ReactorId net) :=
   (exec.reactors id).timer
 
-end Executable
-
-end Network
+end Network.Executable
