Runtime/Network/Execution/Apply.lean
@@ -4,6 +4,7 @@ namespace Network.Executable
 
 def apply (exec : Executable net) (output : ReactionOutput exec) : Executable net := { exec with
   queue := exec.queue.merge output.events
+  state := stateAfter output
   reactors := fun id => { exec.reactors id with
     interface := 
       if      h : id = output.reactor then h ▸ container output -- Updates the output ports of the reaction's container.
@@ -21,5 +22,15 @@ where
   child (output : ReactionOutput exec) (child : ReactorId.Child output.reactor) : (kind : Reactor.InterfaceKind) → kind.interfaceType ((child : ReactorId net).class.interface kind)
     | .inputs => fun var => (output.child var).orElse (fun _ => exec.interface child .inputs var)
     | _       => exec.interface child _
+
+  stateAfter (output : ReactionOutput exec) : Executable.State :=
+    if output.stopRequested then
+      -- When requesting to stop, we need to make sure we don't override
+      -- if we're already in the process of shutting down.
+      match exec.state with
+      | .executing | .stopRequested => .stopRequested
+      | .shuttingDown               => .shuttingDown
+    else
+      exec.state
 
 end Network.Executable
